src/array/FArray.v
@@ -925,7 +925,7 @@ Section FArray.
   Variable key_comp : Comparable key.
   Variable elt_ord : OrdType elt.
   Variable elt_comp : Comparable elt.
-  (* Variable key_inh :  Inhabited key. *)
+  Variable key_inh :  Inhabited key.
   Variable elt_inh :  Inhabited elt.
 
   Instance key_dec : DecType key := @EqbToDecType _ Comparable2EqbType.
@@ -1428,6 +1428,7 @@ Section FArray.
 
   Lemma raw_add_d_rem : forall m (Hm: Sorted (Raw.ltk key_ord) m) x,
       raw_add_nodefault x default_value m = Raw.remove key_comp x m.
+  Proof.
     intros m Hm x.
     unfold raw_add_nodefault.
     rewrite cmp_refl.
@@ -1446,7 +1447,7 @@ Section FArray.
               + intro. contradiction.
               + intro. contradict H0.
                 apply Raw.remove_1; auto.
-            - apply Raw.remove_4; auto. eapply EqbToDecType.
+            - apply Raw.remove_4; auto. apply (@EqbToDecType _ Comparable2EqbType).
           }
         * { intros k e e' H0 H1.
             destruct (eq_dec x k) as [e0|n].
@@ -1456,9 +1457,10 @@ Section FArray.
               + contradict H2.
                 apply Raw.remove_1; auto.
               + apply key_comp.
+              + apply (@EqbToDecType _ Comparable2EqbType).
             - apply (Raw.remove_2 key_comp Hm n) in H0.
               specialize (Raw.remove_sorted key_comp Hm x). intros H2.
-              specialize (Raw.MapsTo_inj key_dec H2 H0 H1).
+              specialize (Raw.MapsTo_inj H2 H0 H1).
               intro H3. subst. apply cmp_refl.
           }
   Qed.
@@ -1480,19 +1482,19 @@ Section FArray.
   Lemma add_eq_d : forall m x y,
       x = y -> find y (add x default_value m) = None.
   Proof.
-    intros.
-    simpl.
+    intros m x y h.
     rewrite add_d_rem.
     case_eq (find y (remove x m)); auto.
-    intros.
+    intros e H0.
     apply find_2 in H0.
     unfold MapsTo, Raw.MapsTo in H0.
-    assert (exists e, InA (Raw.eqk (elt:=elt)) (y, e) (remove x m).(this)).
-    exists e. apply Raw.InA_eqke_eqk in H0. auto.
+    assert (H1:exists e, InA (Raw.eqk (elt:=elt)) (y, e) (remove x m).(this)).
+    { exists e. apply Raw.InA_eqke_eqk in H0. auto. }
     rewrite <- Raw.In_alt in H1; auto.
-    contradict H1.
-    apply remove_1; auto.
-    apply key_comp.
+    - contradict H1.
+      apply remove_1; auto.
+    - apply key_comp.
+    - apply (@EqbToDecType _ Comparable2EqbType).
   Qed.
 
   Lemma add_neq_o : forall m x y e,
@@ -1547,8 +1549,8 @@ Section FArray.
   Lemma Equiv_Equivb : forall m m', Equiv m m' <-> Equivb m m'.
   Proof.
     unfold Equiv, Equivb, Raw.Equivb, cmp; intuition; specialize (H1 k e e' H H2).
-    destruct (compare e e'); auto; apply lt_not_eq in l; auto.
-    destruct (compare e e'); auto; now contradict H1.
+    - unfold compare2eqb; destruct (compare e e'); auto; apply lt_not_eq in l; auto.
+    - unfold compare2eqb in *; destruct (compare e e'); auto; inversion H1.
   Qed.
 
   (** Composition of the two last results: relation between [Equal]
@@ -1574,17 +1576,17 @@ Section FArray.
   Proof.
     intros a i j v Heq.
     unfold select, store.
-    case_eq (cmp v default_value); intro; auto.
-    unfold cmp in H.
-    case (compare v default_value) in H; auto; try now contradict H.
-    rewrite e.
-    rewrite add_eq_d; auto.
-    assert (v <> default_value).
-    unfold cmp in H.
-    case (compare v default_value) in H; auto; try now contradict H.
-    apply lt_not_eq in l. auto.
-    apply lt_not_eq in l. auto.
-    rewrite (add_eq_o a Heq H0). auto.
+    case_eq (cmp v default_value); intro H; auto.
+    - unfold cmp, compare2eqb in H.
+      case (compare v default_value) as [ | |e] in H; auto; try now contradict H.
+      rewrite e.
+      rewrite add_eq_d; auto.
+    - assert (H0: v <> default_value).
+      { unfold cmp, compare2eqb in H.
+        case (compare v default_value) as [l|e|l] in H; auto; try now contradict H.
+        - apply lt_not_eq in l. auto.
+        - apply lt_not_eq in l. auto. }
+      rewrite (add_eq_o a Heq H0). auto.
   Qed.
 
   Lemma read_over_write : forall a i v, select (store a i v) i = v.
@@ -1733,7 +1735,7 @@ Section FArray.
                  a <> b -> {i : key | select a i <> select b i}).
       {
         clear a b. intros x y.
-        case_eq (list_eq_dec (@eq_dec _ (Raw.ke_dec key_dec elt_dec)) x y).
+        case_eq (list_eq_dec (@eq_dec _ (Raw.ke_dec key_comp (@EqbToDecType _ Comparable2EqbType))) x y).
         - intros e He. subst x. intros xS yS xD yD a b. subst a b.
           rewrite (proof_irrelevance _ xS yS),  (proof_irrelevance _ xD yD).
           intro H. elim H. reflexivity.
@@ -1825,7 +1827,8 @@ Section FArray.
     Qed.
 
     Definition diff (a b: farray) : key.
-      case_eq (equal a b); intro.
+    Proof.
+      case_eq (equal a b); intro H.
       - apply default_value.
       - apply (diff_index (notequal_neq H)).
     Defined.
@@ -1850,16 +1853,16 @@ End FArray.
 
 Arguments farray _ _ {_} {_}.
 Arguments select {_} {_} {_} {_} {_} _ _.
-Arguments store {_} {_} {_} {_} {_} {_} {_} {_} _ _ _.
-Arguments diff {_} {_} {_} {_} {_} {_} {_} {_} {_} {_} _ _.
+Arguments store {_} {_} {_} {_} {_} {_} {_} _ _ _.
+Arguments diff {_} {_} {_} {_} {_} {_} {_} {_} _ _.
 Arguments equal {_} {_} {_} {_} {_} {_} {_}  _ _.
 Arguments equal_iff_eq {_} {_} {_} {_} {_} {_} {_} _ _.
-Arguments read_over_same_write {_} {_} {_} {_} {_} {_} {_} {_} {_} _ _ _ _ _.
-Arguments read_over_write {_} {_} {_} {_} {_} {_} {_} {_} {_} _ _ _.
-Arguments read_over_other_write {_} {_} {_} {_} {_} {_} {_} {_} _ _ _ _ _.
-Arguments extensionality {_} {_} {_} {_} {_} {_} {_} {_} {_} _ _ _.
+Arguments read_over_same_write {_} {_} {_} {_} {_} {_} {_} _ _ _ _ _.
+Arguments read_over_write {_} {_} {_} {_} {_} {_} {_} _ _ _.
+Arguments read_over_other_write {_} {_} {_} {_} {_} {_} _ _ _ _ _.
+Arguments extensionality {_} {_} {_} {_} {_} {_} {_} _ _ _.
 Arguments extensionality2 {_} {_} {_} {_} {_} {_} {_} {_} {_} _.
-Arguments select_at_diff {_} {_} {_} {_} {_} {_} {_} {_} {_} {_} {_} _ _ _.
+Arguments select_at_diff {_} {_} {_} {_} {_} {_} {_} {_} {_} _ _ _.
 
 
 Notation "a '[' i ']'" := (select a i) (at level 1, format "a [ i ]") : farray_scope.
