src/classes/SMT_classes_instances.v
@@ -19,18 +19,11 @@ Require Export SMT_classes.
 
 Section Unit.
 
-  Let eqb : unit -> unit -> bool := fun _ _ => true.
-
   Let lt : unit -> unit -> Prop := fun _ _ => False.
-  
+
   Instance unit_ord : OrdType unit.
   Proof. exists lt; unfold lt; trivial.
     intros; contradict H; trivial.
-  Defined.
-
-  Instance unit_eqbtype : EqbType unit.
-  Proof.
-    exists eqb. intros. destruct x, y. unfold eqb. split; trivial.
   Defined.
 
   Instance unit_comp : @Comparable unit unit_ord.
@@ -39,24 +32,18 @@ Section Unit.
     apply OrderedType.EQ; trivial.
   Defined.
 
+  Instance unit_eqbtype : EqbType unit := Comparable2EqbType.
+
   Instance unit_inh : Inhabited unit := {| default_value := tt |}.
-  
+
   Instance unit_compdec : CompDec unit := {|
-    Eqb := unit_eqbtype;
     Ordered := unit_ord;
     Comp := unit_comp;
     Inh := unit_inh
   |}.
 
-
-  
   Definition unit_typ_compdec := Typ_compdec unit unit_compdec.
 
-
-  Lemma eqb_eq_unit : forall x y, eqb x y <-> x = y.
-  Proof. intros. split; case x; case y; unfold eqb; intros; now auto.
-  Qed.
-  
 End Unit.
 
 
@@ -65,21 +52,15 @@ Section Bool.
   Definition ltb_bool x y := negb x && y.
 
   Definition lt_bool x y := ltb_bool x y = true.
-  
+
   Instance bool_ord : OrdType bool.
   Proof.
     exists lt_bool.
     intros x y z.
-    case x; case y; case z; intros; simpl; subst; auto. 
+    case x; case y; case z; intros; simpl; subst; auto.
     intros x y.
-    case x; case y; intros; simpl in H; easy. 
+    case x; case y; intros; simpl in H; easy.
   Defined.
-
-  Instance bool_eqbtype : EqbType bool :=
-    {| eqb := Bool.eqb; eqb_spec := eqb_true_iff |}.
-  
-  Instance bool_dec : DecType bool :=
-    EqbToDecType _ bool_eqbtype.
 
   Instance bool_comp: Comparable bool.
   Proof.
@@ -99,11 +80,14 @@ Section Bool.
     case x in *; case y in *; auto.
   Defined.
 
+  Instance bool_eqbtype : EqbType bool := Comparable2EqbType.
+
+  Instance bool_dec : DecType bool := EqbToDecType.
+
   Instance bool_inh : Inhabited bool := {| default_value := false|}.
 
   Instance bool_compdec : CompDec bool := {|
-    Eqb := bool_eqbtype;                                    
-    Ordered := bool_ord;                                    
+    Ordered := bool_ord;
     Comp := bool_comp;
     Inh := bool_inh
   |}.
@@ -126,29 +110,23 @@ Section Z.
     exact Z_as_OT.lt_not_eq.
   Defined.
 
-  Instance Z_eqbtype : EqbType Z :=
-    {| eqb := Z.eqb; eqb_spec := Z.eqb_eq |}.
 
-  (* Instance Z_eqbtype : EqbType Z := *)
-  (*   {| eqb := Zeq_bool; eqb_spec := fun x y => symmetry (Zeq_is_eq_bool x y) |}. *)
-  
-  Instance Z_dec : DecType Z :=
-    EqbToDecType _ Z_eqbtype.
-
-  
   Instance Z_comp: Comparable Z.
   Proof.
     constructor.
     apply Z_as_OT.compare.
   Defined.
 
+  Instance Z_eqbtype : EqbType Z := Comparable2EqbType.
+
+  Instance Z_dec : DecType Z := EqbToDecType.
+
 
   Instance Z_inh : Inhabited Z := {| default_value := 0%Z |}.
 
-    
+
   Instance Z_compdec : CompDec Z := {|
-    Eqb := Z_eqbtype;                                    
-    Ordered := Z_ord;                                    
+    Ordered := Z_ord;
     Comp := Z_comp;
     Inh := Z_inh
   |}.
@@ -202,7 +180,7 @@ Section Z.
 
   Lemma lt_Z_B2P': forall x y, ltP_Z x y <-> Z.lt x y.
   Proof. intros x y; split; intro H.
-         unfold ltP_Z in H. 
+         unfold ltP_Z in H.
          case_eq ((x <? y)%Z ); intros; rewrite H0 in H; try easy.
          now apply Z.ltb_lt in H0.
          apply lt_Z_B2P.
@@ -211,7 +189,7 @@ Section Z.
 
   Lemma le_Z_B2P': forall x y, leP_Z x y <-> Z.le x y.
   Proof. intros x y; split; intro H.
-         unfold leP_Z in H. 
+         unfold leP_Z in H.
          case_eq ((x <=? y)%Z ); intros; rewrite H0 in H; try easy.
          now apply Z.leb_le in H0.
          apply le_Z_B2P.
@@ -220,7 +198,7 @@ Section Z.
 
   Lemma gt_Z_B2P': forall x y, gtP_Z x y <-> Z.gt x y.
   Proof. intros x y; split; intro H.
-         unfold gtP_Z in H. 
+         unfold gtP_Z in H.
          case_eq ((x >? y)%Z ); intros; rewrite H0 in H; try easy.
          now apply Zgt_is_gt_bool in H0.
          apply gt_Z_B2P.
@@ -229,7 +207,7 @@ Section Z.
 
   Lemma ge_Z_B2P': forall x y, geP_Z x y <-> Z.ge x y.
   Proof. intros x y; split; intro H.
-         unfold geP_Z in H. 
+         unfold geP_Z in H.
          case_eq ((x >=? y)%Z ); intros; rewrite H0 in H; try easy.
          rewrite Z.geb_leb in H0. rewrite le_Z_B2P in H0.
          apply le_Z_B2P' in H0. now apply Z.ge_le_iff.
@@ -252,32 +230,29 @@ Section Nat.
 
   Instance Nat_ord : OrdType nat.
   Proof.
-    
+
     exists Nat_as_OT.lt.
     exact Nat_as_OT.lt_trans.
     exact Nat_as_OT.lt_not_eq.
   Defined.
 
-  Instance Nat_eqbtype : EqbType nat :=
-    {| eqb := Structures.nat_eqb; eqb_spec := Structures.nat_eqb_eq |}.
-  
-  Instance Nat_dec : DecType nat :=
-    EqbToDecType _ Nat_eqbtype.
 
-  
   Instance Nat_comp: Comparable nat.
   Proof.
     constructor.
     apply Nat_as_OT.compare.
   Defined.
 
+  Instance Nat_eqbtype : EqbType nat := Comparable2EqbType.
+
+  Instance Nat_dec : DecType nat := EqbToDecType.
+
 
   Instance Nat_inh : Inhabited nat := {| default_value := O%nat |}.
 
-    
+
   Instance Nat_compdec : CompDec nat := {|
-    Eqb := Nat_eqbtype;                                    
-    Ordered := Nat_ord;                                    
+    Ordered := Nat_ord;
     Comp := Nat_comp;
     Inh := Nat_inh
   |}.
@@ -294,23 +269,20 @@ Section Positive.
     exact Positive_as_OT.lt_not_eq.
   Defined.
 
-  Instance Positive_eqbtype : EqbType positive :=
-    {| eqb := Pos.eqb; eqb_spec := Pos.eqb_eq |}.
-  
-  Instance Positive_dec : DecType positive :=
-    EqbToDecType _ Positive_eqbtype.
-
   Instance Positive_comp: Comparable positive.
   Proof.
     constructor.
     apply Positive_as_OT.compare.
   Defined.
 
+  Instance Positive_eqbtype : EqbType positive := Comparable2EqbType.
+
+  Instance Positive_dec : DecType positive := EqbToDecType.
+
   Instance Positive_inh : Inhabited positive := {| default_value := 1%positive |}.
 
   Instance Positive_compdec : CompDec positive := {|
-    Eqb := Positive_eqbtype;                                    
-    Ordered := Positive_ord;                                    
+    Ordered := Positive_ord;
     Comp := Positive_comp;
     Inh := Positive_inh
   |}.
@@ -323,7 +295,7 @@ Section BV.
 
   Import BITVECTOR_LIST.
 
-  
+
   Instance BV_ord n : OrdType (bitvector n).
   Proof.
     exists (fun a b => (bv_ult a b)).
@@ -342,14 +314,7 @@ Section BV.
     apply H. easy.
   Defined.
 
-  Instance BV_eqbtype n : EqbType (bitvector n) :=
-    {| eqb := @bv_eq n;
-       eqb_spec := @bv_eq_reflect n |}.
 
-  Instance BV_dec n : DecType (bitvector n) :=
-    EqbToDecType _ (BV_eqbtype n).
-
-  
   Instance BV_comp n: Comparable (bitvector n).
   Proof.
     constructor.
@@ -388,13 +353,16 @@ Section BV.
     now apply RAWBITVECTOR_LIST.rev_neq in H.
   Defined.
 
+  Instance BV_eqbtype n : EqbType (bitvector n) := Comparable2EqbType.
+
+  Instance BV_dec n : DecType (bitvector n) := EqbToDecType.
+
   Instance BV_inh n : Inhabited (bitvector n) :=
     {| default_value := zeros n |}.
 
 
   Instance BV_compdec n: CompDec (bitvector n) := {|
-    Eqb := BV_eqbtype n;                                    
-    Ordered := BV_ord n;                                    
+    Ordered := BV_ord n;
     Comp := BV_comp n;
     Inh := BV_inh n
   |}.
@@ -408,7 +376,6 @@ Section FArray.
   Instance FArray_ord key elt
            `{key_ord: OrdType key}
            `{elt_ord: OrdType elt}
-           `{elt_dec: DecType elt}
            `{elt_inh: Inhabited elt}
            `{key_comp: @Comparable key key_ord} : OrdType (farray key elt).
   Proof.
@@ -419,49 +386,20 @@ Section FArray.
     apply lt_farray_not_eq in H.
     apply H.
     rewrite H0.
-    apply eqfarray_refl. auto.
+    apply eqfarray_refl.
   Defined.
 
-  Instance FArray_eqbtype key elt
-           `{key_ord: OrdType key}
-           `{elt_ord: OrdType elt}
-           `{elt_eqbtype: EqbType elt}
-           `{key_comp: @Comparable key key_ord}
-           `{elt_comp: @Comparable elt elt_ord}
-           `{elt_inh: Inhabited elt}
-    : EqbType (farray key elt).
-  Proof.
-    exists FArray.equal.
-    intros.
-    split.
-    apply FArray.equal_eq.
-    intros. subst. apply eq_equal. apply eqfarray_refl.
-    apply EqbToDecType. auto.
-  Defined.
 
-  
-  Instance FArray_dec key elt
-           `{key_ord: OrdType key}
-           `{elt_ord: OrdType elt}
-           `{elt_eqbtype: EqbType elt}
-           `{key_comp: @Comparable key key_ord}
-           `{elt_comp: @Comparable elt elt_ord}
-           `{elt_inh: Inhabited elt}
-    : DecType (farray key elt) :=
-    EqbToDecType _ (FArray_eqbtype key elt).
-
-  
   Instance FArray_comp key elt
            `{key_ord: OrdType key}
            `{elt_ord: OrdType elt}
-           `{elt_eqbtype: EqbType elt}
            `{key_comp: @Comparable key key_ord}
            `{elt_inh: Inhabited elt}
            `{elt_comp: @Comparable elt elt_ord} : Comparable (farray key elt).
   Proof.
     constructor.
     intros.
-    destruct (compare_farray key_comp (EqbToDecType _ elt_eqbtype) elt_comp x y).
+    destruct (compare_farray key_comp elt_comp x y).
     - apply OrderedType.LT. auto.
     - apply OrderedType.EQ.
       specialize (@eq_equal key elt key_ord key_comp elt_ord elt_comp elt_inh x y).
@@ -470,6 +408,23 @@ Section FArray.
       now apply equal_eq in e.
     - apply OrderedType.GT. auto.
   Defined.
+
+  Instance FArray_eqbtype key elt
+           `{key_ord: OrdType key}
+           `{elt_ord: OrdType elt}
+           `{key_comp: @Comparable key key_ord}
+           `{elt_comp: @Comparable elt elt_ord}
+           `{elt_inh: Inhabited elt}
+    : EqbType (farray key elt) := Comparable2EqbType.
+
+
+  Instance FArray_dec key elt
+           `{key_ord: OrdType key}
+           `{elt_ord: OrdType elt}
+           `{key_comp: @Comparable key key_ord}
+           `{elt_comp: @Comparable elt elt_ord}
+           `{elt_inh: Inhabited elt}
+    : DecType (farray key elt) := EqbToDecType.
 
   Instance FArray_inh key elt
            `{key_ord: OrdType key}
@@ -482,42 +437,25 @@ Section FArray.
           `{elt_compdec: CompDec elt} :
     CompDec (farray key elt) :=
     {|
-      Eqb := FArray_eqbtype key elt;
       Ordered := FArray_ord key elt;
-      (*  Comp := FArray_comp key elt ; *)
+      Comp := FArray_comp key elt ;
       Inh := FArray_inh key elt
     |}.
-  
-  Next Obligation.
-    constructor.
-    destruct key_compdec, elt_compdec.
-    simpl in *.
-    unfold lt_farray.
-    intros. simpl.
-    unfold EqbToDecType. simpl.
-    case_eq (compare x y); intros.
-    apply OrderedType.LT.
-    destruct (compare x y); try discriminate H; auto.
-    apply OrderedType.EQ.
-    destruct (compare x y); try discriminate H; auto.
-    apply OrderedType.GT.
-    destruct (compare y x); try discriminate H; auto; clear H.
-  Defined.
 
 End FArray.
 
 
 Section Int63.
-  
+
   Local Open Scope int63_scope.
 
   Let int_lt x y :=
     if Int63Native.ltb x y then True else False.
-  
+
   Instance int63_ord : OrdType int.
   Proof.
     exists int_lt; unfold int_lt.
-    - intros x y z. 
+    - intros x y z.
       case_eq (x < y); intro;
         case_eq (y < z); intro;
           case_eq (x < z); intro;
@@ -533,12 +471,6 @@ Section Int63.
       rewrite <- Int63Properties.to_Z_eq.
       exact (Z.lt_neq _ _ H).
   Defined.
-  
-  Instance int63_eqbtype : EqbType int :=
-    {| eqb := Int63Native.eqb; eqb_spec := Int63Properties.eqb_spec |}.
-
-  Instance int63_dec : DecType int :=
-    EqbToDecType _ int63_eqbtype.
 
 
   Instance int63_comp: Comparable int.
@@ -566,16 +498,19 @@ Section Int63.
       rewrite H0. auto.
   Defined.
 
+  Instance int63_eqbtype : EqbType int := Comparable2EqbType.
+
+  Instance int63_dec : DecType int := EqbToDecType.
+
 
   Instance int63_inh : Inhabited int := {| default_value := 0 |}.
-    
+
   Instance int63_compdec : CompDec int := {|
-    Eqb := int63_eqbtype;                                    
-    Ordered := int63_ord;                                    
+    Ordered := int63_ord;
     Comp := int63_comp;
     Inh := int63_inh
   |}.
-         
+
 
 End Int63.
 
@@ -584,25 +519,6 @@ Section option.
 
   Generalizable Variable A.
   Context `{HA : CompDec A}.
-
-
-  Definition option_eqb (x y : option A) : bool :=
-    match x, y with
-    | Some a, Some b => eqb a b
-    | None, None => true
-    | _, _ => false
-    end.
-
-
-  Lemma option_eqb_spec : forall (x y : option A), option_eqb x y = true <-> x = y.
-  Proof.
-    intros [a| ] [b| ]; simpl; split; try discriminate; auto.
-    - intro H. rewrite eqb_spec in H. now subst b.
-    - intros H. inversion H as [H1]. now rewrite eqb_spec.
-  Qed.
-
-
-  Instance option_eqbtype : EqbType (option A) := Build_EqbType _ _ option_eqb_spec.
 
 
   Definition option_lt (x y : option A) : Prop :=
@@ -647,15 +563,15 @@ Section option.
     - now apply EQ.
   Defined.
 
-
   Instance option_comp : Comparable (option A) := Build_Comparable _ _ option_compare.
+
+  Instance option_eqbtype : EqbType (option A) := Comparable2EqbType.
 
 
   Instance option_inh : Inhabited (option A) := Build_Inhabited _ None.
 
 
   Instance option_compdec : CompDec (option A) := {|
-    Eqb := option_eqbtype;
     Ordered := option_ord;
     Comp := option_comp;
     Inh := option_inh
@@ -670,27 +586,6 @@ Section list.
   Context `{HA : CompDec A}.
 
 
-  Fixpoint list_eqb (xs ys : list A) : bool :=
-    match xs, ys with
-    | nil, nil => true
-    | x::xs, y::ys => eqb x y && list_eqb xs ys
-    | _, _ => false
-    end.
-
-
-  Lemma list_eqb_spec : forall (x y : list A), list_eqb x y = true <-> x = y.
-  Proof.
-    induction x as [ |x xs IHxs]; intros [ |y ys]; simpl; split; try discriminate; auto.
-    - rewrite andb_true_iff. intros [H1 H2]. rewrite eqb_spec in H1. rewrite IHxs in H2. now subst.
-    - intros H. inversion H as [H1]. rewrite andb_true_iff; split.
-      + now rewrite eqb_spec.
-      + subst ys. now rewrite IHxs.
-  Qed.
-
-
-  Instance list_eqbtype : EqbType (list A) := Build_EqbType _ _ list_eqb_spec.
-
-
   Fixpoint list_lt (xs ys : list A) : Prop :=
     match xs, ys with
     | nil, nil => False
@@ -698,35 +593,6 @@ Section list.
     | _::_, nil => False
     | x::xs, y::ys => (lt x y) \/ (eqb x y /\ list_lt xs ys)
     end.
-
-
-  Lemma list_lt_trans : forall (x y z : list A),
-      list_lt x y -> list_lt y z -> list_lt x z.
-  Proof.
-    induction x as [ |x xs IHxs]; intros [ |y ys] [ |z zs]; simpl; auto.
-    - inversion 1.
-    - intros [H1|[H1a H1b]] [H2|[H2a H2b]].
-      + left; eapply lt_trans; eauto.
-      + left. unfold is_true in H2a. rewrite eqb_spec in H2a. now subst z.
-      + left. unfold is_true in H1a. rewrite eqb_spec in H1a. now subst y.
-      + right. split.
-        * unfold is_true in H1a. rewrite eqb_spec in H1a. now subst y.
-        * eapply IHxs; eauto.
-  Qed.
-
-
-  Lemma list_lt_not_eq : forall (x y : list A), list_lt x y -> x <> y.
-  Proof.
-    induction x as [ |x xs IHxs]; intros [ |y ys]; simpl; auto.
-    - discriminate.
-    - intros [H1|[H1 H2]]; intros H; inversion H; subst.
-      + eapply lt_not_eq; eauto.
-      + eapply IHxs; eauto.
-  Qed.
-
-
-  Instance list_ord : OrdType (list A) :=
-    Build_OrdType _ _ list_lt_trans list_lt_not_eq.
 
 
   Definition list_compare : forall (x y : list A), Compare list_lt Logic.eq x y.
@@ -738,21 +604,51 @@ Section list.
     - case_eq (compare x y); intros l H.
       + apply LT. simpl. now left.
       + case_eq (IHxs ys); intros l1 H1.
-        * apply LT. simpl. right. split; auto. now apply eqb_spec.
+        * apply LT. simpl. right. split; auto. now apply compare2eqb_spec.
         * apply EQ. now rewrite l, l1.
-        * apply GT. simpl. right. split; auto. now apply eqb_spec.
+        * apply GT. simpl. right. split; auto. now apply compare2eqb_spec.
       + apply GT. simpl. now left.
   Defined.
 
 
+  Lemma list_lt_trans : forall (x y z : list A),
+      list_lt x y -> list_lt y z -> list_lt x z.
+  Proof.
+    induction x as [ |x xs IHxs]; intros [ |y ys] [ |z zs]; simpl; auto.
+    - inversion 1.
+    - intros [H1|[H1a H1b]] [H2|[H2a H2b]].
+      + left; eapply lt_trans; eauto.
+      + left. unfold is_true in H2a. rewrite compare2eqb_spec in H2a. now subst z.
+      + left. unfold is_true in H1a. rewrite compare2eqb_spec in H1a. now subst y.
+      + right. split.
+        * unfold is_true in H1a. rewrite compare2eqb_spec in H1a. now subst y.
+        * eapply IHxs; eauto.
+  Qed.
+
+
+  Lemma list_lt_not_eq : forall (x y : list A), list_lt x y -> x <> y.
+  Proof.
+    induction x as [ |x xs IHxs]; intros [ |y ys]; simpl; auto.
+    - discriminate.
+    - intros [H1|[H1 H2]]; intros H; inversion H; subst.
+      + now apply (lt_not_eq _ _ H1).
+      + now apply (IHxs _ H2).
+  Qed.
+
+
+  Instance list_ord : OrdType (list A) :=
+    Build_OrdType _ _ list_lt_trans list_lt_not_eq.
+
+
   Instance list_comp : Comparable (list A) := Build_Comparable _ _ list_compare.
+
+  Instance list_eqbtype : EqbType (list A) := Comparable2EqbType.
 
 
   Instance list_inh : Inhabited (list A) := Build_Inhabited _ nil.
 
 
   Instance list_compdec : CompDec (list A) := {|
-    Eqb := list_eqbtype;
     Ordered := list_ord;
     Comp := list_comp;
     Inh := list_inh
